remove some complexity while working on first proof

example/out/ProcDecExecOk.v
@@ -93,14 +93,15 @@ Record mySimRel (dec : Decoder) (iregs sregs: RegsT): Prop :=
    ide_e2wfifo_regv: fullType type (SyntaxKind D2E) ;
    ide_e2wfifo_validv: bool ;
    ideregv: fullType type (SyntaxKind (Array 32 (Bit DataSz))) ;
-   idesbflagsv: fullType type (SyntaxKind (Array 32 Bool)) ;
+   (* idesbflagsv: fullType type (SyntaxKind (Array 32 Bool)) ; *)
 
    spcv: word PgmSz ;
    sde_e2wfifo_regv: fullType type (SyntaxKind E2W) ;
    sde_e2wfifo_validv: bool ;
    sderegv: (Fin.t 32 -> word DataSz) ;
-   sdesbflagsv: (Fin.t 32 -> bool) ;
+   (* sdesbflagsv: (Fin.t 32 -> bool) ; *)
 
+   Hsde_e2wfifo_validv_false: sde_e2wfifo_validv = false ;
    Hpcinv: decexec_pc_inv ipcv ide_fifo_validv ide_fifo_regv ;
    Hdeinv: decexec_d2e_inv dec pgmv ide_fifo_validv ide_fifo_regv ;
 
@@ -112,24 +113,42 @@ Record mySimRel (dec : Decoder) (iregs sregs: RegsT): Prop :=
 	    :: ("decexec-e2wFifo_valid", existT _ (SyntaxKind Bool) sde_e2wfifo_validv)
       :: ("pgm", existT _ (SyntaxKind (Array NumInstrs (Bit InstrSz))) pgmv)
       :: ("decexec-regs", existT _ (SyntaxKind (Array 32 (Bit DataSz))) sderegv)
-      :: ("decexec-sbFlags", existT _ (SyntaxKind (Array 32 Bool)) sdesbflagsv)
+      (* :: ("decexec-sbFlags", existT _ (SyntaxKind (Array 32 Bool)) sdesbflagsv) *)
+      :: nil ;
+
+   iregs_arith: RegsT ;
+   Hiregs_arith: iregs_arith =
+   ("decexec-d2eFifo_reg", existT _ (SyntaxKind D2E) ide_fifo_regv)
+      :: ("decexec-d2eFifo_valid", existT _ (SyntaxKind Bool) true)
+      :: ("decexec-pc", existT _ (SyntaxKind (Bit PgmSz)) ipcv)
+      :: ("decexec-e2wFifo_reg", existT _ (SyntaxKind E2W) sde_e2wfifo_regv)
+      :: ("decexec-e2wFifo_valid", existT _ (SyntaxKind Bool) false)
+      :: ("pgm", existT _ (SyntaxKind (Array NumInstrs (Bit InstrSz)))
+                          pgm)
+      :: ("decexec-regs", existT _ (SyntaxKind (Array 32 (Bit DataSz))) sderegv)
+      (* :: ("decexec-sbFlags", existT _ (SyntaxKind (Array 32 Bool)) sdesbflagsv) *)
       :: nil ;
 
    Hsregs: sregs =
    ("decexec-e2wFifo_reg", existT (fullType type) (SyntaxKind E2W) sde_e2wfifo_regv)
     :: ("decexec-e2wFifo_valid", existT (fullType type) (SyntaxKind Bool) sde_e2wfifo_validv)
     :: ("decexec-pc", existT (fullType type) (SyntaxKind (Bit PgmSz)) ipcv)
-	  :: ("pgm", existT (fullType type) (SyntaxKind (Array NumInstrs (Bit InstrSz))) pgmv)
-	  :: ("decexec-regs", existT (fullType type) (SyntaxKind (Array 32 (Bit DataSz))) ideregv)
-	  :: ("decexec-sbFlags", existT (fullType type) (SyntaxKind (Array 32 Bool)) idesbflagsv)
+    :: ("pgm", existT (fullType type) (SyntaxKind (Array NumInstrs (Bit InstrSz))) pgmv)
+    :: ("decexec-regs", existT (fullType type) (SyntaxKind (Array 32 (Bit DataSz))) ideregv)
+    (* :: ("decexec-sbFlags", existT (fullType type) (SyntaxKind (Array 32 Bool)) idesbflagsv) *)
+    :: nil ;
+
+   sregs_arith : RegsT ;
+   Hsregs_arith: sregs_arith =
+   ("decexec-e2wFifo_reg", existT (fullType type) (SyntaxKind E2W) sde_e2wfifo_regv)
+    :: ("decexec-e2wFifo_valid", existT (fullType type) (SyntaxKind Bool) false)
+    :: ("decexec-pc", existT (fullType type) (SyntaxKind (Bit PgmSz)) ipcv)
+    :: ("pgm", existT (fullType type) (SyntaxKind (Array NumInstrs (Bit InstrSz))) pgmv)
+    :: ("decexec-regs", existT (fullType type) (SyntaxKind (Array 32 (Bit DataSz))) ideregv)
+    (* :: ("decexec-sbFlags", existT (fullType type) (SyntaxKind (Array 32 Bool)) idesbflagsv) *)
     :: nil
 
  }.
-Check fullType.
-Check type.
-Compute (fullType type (SyntaxKind D2E)).
-Compute (fullType type (SyntaxKind (Array NumInstrs (Bit InstrSz)))).
-Check mySimRel.
 
 
 Section DecExecSepOk.
@@ -164,14 +183,6 @@ Ltac exists_uspec :=
    | [ H: mySimRel _ _ _ |- _ ] => destruct H
    | [ |- mySimRel ?dec ?iregs ?sregs ] => idtac "mySimRel" ; destruct mySimRel
    | [ |- SemAction _ _ _ _ _ _ ] => idtac "semaction" ; discharge_SemAction
-   (* | [ |- In ("decexec-e2wFifo_valid", _) _ ] => admit
-   | [ |- In ("decexec-e2wFifo_reg", _) _ ] => admit
-   | [ |- In ("decexec-pc", _) _ ] => admit
-   | [ |- In ("decexec-sbFlags", _) _ ] => idtac "sbflags"; admit (* something wrong *)
-   | [ |- In ("decexec-pc", _) _ ] => admit
-   | [ |- In ("decexec-regs", _) _ ] => admit
-   | [ |- In ("decexec-sbFlags", _) (getKindAttr _) ] => admit
-   | [ |- In ("pgm", _) _ ] => admit *)
    | [ |- findReg _ (_ :: _) = _ ] => unfold findReg
    | [ H3: fst ?x = _ |- (if string_dec ?m (fst ?x) then _ else _) = _ ] => idtac "fstx"; idtac x ; rewrite H3 
    end.
@@ -181,16 +192,44 @@ Ltac discharge_findreg :=
    | [ |- findReg _ _ = _ ] => idtac "findreg"; unfold findReg 
    end; repeat discharge_string_dec.
 
+Ltac discharge_simulationZero mySimRel :=
+  apply _simulationZeroAction with (simRel := mySimRel) ; auto; simpl; intros;
+  (repeat match goal with
+          | H: _ \/ _ |- _ => destruct H
+          | H: False |- _ => exfalso; apply H
+          | H: (?a, ?b) = (?c, ?d) |- _ =>
+            let H2 := fresh in
+            inversion H;
+            pose proof (f_equal snd H) as H2 ;
+            simpl in H2; subst; clear H; EqDep_subst
+         | H: SemAction _ (convertLetExprSyntax_ActionT ?e) _ _ _ _ |- _ =>
+           apply convertLetExprSyntax_ActionT_full in H; dest; subst
+          | H: SemAction _ _ _ _ _ _ |- _ =>
+            apply inversionSemAction in H; dest; subst
+          | H: if ?P then _ else _ |- _ => case_eq P; let i := fresh in intros i; rewrite ?i in *; dest
+          | H: Forall2 _ _ _ |- _ => inv H
+          | H: ?a = ?a |- _ => clear H
+          | H: match convertLetExprSyntax_ActionT ?P with
+               | _ => _
+               end |- _ =>
+            case_eq P; intros;
+            match goal with
+            | H': P = _ |- _ => rewrite ?H' in *; simpl in *; try discriminate
+            end
+          end) ; dest; simpl in *; repeat subst; simpl in *.
+
+Ltac andb_true_intro_split := apply andb_true_intro; split.
 Theorem decexecSep_ok:
     TraceInclusion decexecSepWf
                    decexecWf.
   Proof.
   discharge_appendage.
-  discharge_simulationGeneral (mySimRel decoder) ltac:(discharge_DisjKey).
-  + discharge_NoSelfCall.
+  discharge_simulationZero (mySimRel decoder).
+  (* discharge_simulationGeneral (mySimRel decoder) ltac:(discharge_DisjKey).
+  + discharge_NoSelfCall. *)
   + destruct H. rewrite Hsregs. unfold getKindAttr. simpl. reflexivity.
   + destruct H. rewrite Hiregs. unfold getKindAttr. simpl. reflexivity.
-  + exists (x2 :: x3 :: x1 :: x4 :: x5 :: x6 :: nil). split.
+  + exists (x2 :: x3 :: x1 :: x4 :: x5 (* :: x6 *) :: nil). split.
    ++ repeat apply Forall2_cons; simpl; try (split; [try congruence | eexists; eauto]).
       apply Forall2_nil.
    ++ repeat match goal with
@@ -199,43 +238,24 @@ Theorem decexecSep_ok:
                               let m3 := fresh "v" in destruct H as [m1 [m2 m3]]
             end; simpl in *; subst.
            econstructor; try repeat f_equal; eauto.
-    * unfold decexec_pc_inv; rewrite H13. left; reflexivity. 
-    * unfold decexec_d2e_inv. rewrite H13. left; reflexivity.
+    * unfold decexec_pc_inv. rewrite (* H13 *) H11. left; reflexivity. 
+    * unfold decexec_d2e_inv. rewrite (* H13 *) H11. left; reflexivity.
   + right. exists "decexec-decexecArith". eexists. split.
     * left. trivial.
-    * destruct H1. exists oImp; eexists. rewrite Hiregs. split.
+    * destruct H1. exists sregs_arith; rewrite Hsregs_arith. eexists. rewrite Hsregs. split.
       ** discharge_SemAction. (* getbool something *)
+      *** repeat andb_true_intro_split. 
+       ++ admit.
+       ++ (* admit.
+       ++ admit.
+       ++ *) apply negb_true_iff. rewrite <- Hsde_e2wfifo_validv_false. reflexivity.
       *** admit.
-      *** admit.
-      *** 
-    ** admit. (* this looks wrong *)
-    ** admit. (* this looks wrong *)
-    ** admit. (* mySimRel doUpdRegs tactic needed *)
-  + right. exists "decexec-decexecLd". eexists. split.
-    * right. left. trivial.
-    * exists oSpec. repeat exists_uspec.
-      ** admit.
-      ** simpl. admit.
-      ** admit.
-      ** admit.
-      ** admit.
-  + right. exists "decexec-decexecSt". eexists. split.
-    * right. right. left. trivial.
-    * exists oImp. repeat exists_uspec.
-unfold mySimRel in H1. destruct H1. destruct a. destruct d. destruct Hdeinv, Hpcinv.
-
-      ** admit. (* getOp instr == 2 && d2efifo_valid *)
-      ** simpl. trivial. (* FIXME nil = _ :: nil *) admit.
-      **  admit.
-      ** admit.
-      ** admit.
-  + right. exists "decexec-decexecToHost". eexists. split.
-   * right. right. right. left. trivial.
-   * exists oSpec. repeat exists_uspec.
-     ** simpl. Search (_ && _). admit.
-     ** admit.
-     ** simpl.  admit.
-     ** (* FIXME oSPEC missing decexec-e2wFifo_reg *) admit.
-     ** admit.
-     ** admit.
+    ** repeat match goal with
+            | H: RegT |- _ => let m1 := fresh "nm" in
+                              let m2 := fresh "knd" in
+                              let m3 := fresh "v" in destruct H as [m1 [m2 m3]]
+            end; simpl in *; subst.
+       admit.
+  + admit. 
 Admitted.
+End DecExecSepOk.
