example/out/ProcDecExec.v
@@ -21,7 +21,7 @@ Module module'mkDecExec.
     Variable exec: Decoder.Executer.
         (* method bindings *)
     Let pc : string := instancePrefix--"pc".
-    Let sbFlags : string := instancePrefix--"sbFlags".
+    (* Let sbFlags : string := instancePrefix--"sbFlags". *)
     Let rf: string := instancePrefix--"regs".
     Let mem: string := instancePrefix--"mem".
     Let pgm: string := "pgm".
@@ -40,99 +40,36 @@ Module module'mkDecExec.
     with Register pc : Bit PgmSz <- natToWord PgmSz 0
     with Register pgm : Array NumInstrs (Bit InstrSz) <- Default
     with Register rf : Array NumRegs (Bit DataSz) <- Default
-    with Register sbFlags : Array NumRegs Bool <- Default
+    (* with Register sbFlags : Array NumRegs Bool <- Default *)
     with Rule instancePrefix--"decexecArith" :=
     (
         Read e2wFifo_valid_v : Bool <- e2wFifo_valid ;
         Read pc_v : Bit PgmSz <- pc ;
-        Read sbFlags_v : Array NumRegs Bool <- sbFlags ;
+        (* Read sbFlags_v : Array NumRegs Bool <- sbFlags ; *)
        Read instrs : Array NumInstrs (Bit InstrSz) <- pgm ;
-       LET call17 : Bit InstrSz <- #instrs @[  #pc_v ] ;
-       LET isOpArith : Bool <- (getOp dec _ call17) == $$opArith ;
-       LET inst : Bit InstrSz <- #instrs @[ #pc_v ] ;
+       LET inst : Bit InstrSz <- #instrs @[  #pc_v ] ;
+       LET isOpArith : Bool <- (getOp dec _ inst) == $$opArith ;
        LET src1 : Bit RegFileSz <-  getSrc1 dec _ inst ;
        LET src2 : Bit RegFileSz <-  getSrc2 dec _ inst ;
 
-        Assert((((#isOpArith && (!(#sbFlags_v @[ #src1 ]))) && (!(#sbFlags_v @[ #src2 ]))) && (!#e2wFifo_valid_v))) ;
+        Assert(#isOpArith 
+	(* && !(#sbFlags_v @[ #src1 ]) *)
+	(* && (!(#sbFlags_v @[ #src2 ])) *)
+	 && (!#e2wFifo_valid_v)) ;
        LET dst : Bit RegFileSz (* varbinding *) <-  getDst dec _ inst ;
        LET arithOp : OpArithK (* varbinding *) <- getArithOp dec _ inst ;
        Read regsval : Array NumRegs (Bit DataSz) <- rf ;
        LET val1 : Bit DataSz (* varbinding *) <-  #regsval @[ #src1 ] ;
        LET val2 : Bit DataSz (* varbinding *) <-  #regsval @[ #src2 ] ;
        LET execVal : Bit DataSz <- (execArith exec _ arithOp val1 val2) ;
-               LET flags : Array NumRegs Bool (* non-call varbinding *) <- #sbFlags_v ;
+       (* LET flags : Array NumRegs Bool (* non-call varbinding *) <- #sbFlags_v ;
                LET flags : Array NumRegs Bool <- #flags @[#dst <- $$true] ;
-               Write sbFlags : Array NumRegs Bool <- #flags ;
+               Write sbFlags : Array NumRegs Bool <- #flags ; *)
                LET e2w : E2W (* non-call varbinding *) <- STRUCT { "idx" ::= (#dst) ; "val" ::= (#execVal)  }%kami_expr ;
                Write e2wFifo_reg : E2W <- #e2w ;
                Write e2wFifo_valid : Bool <- ($$true)%kami_expr ;
                Write pc : Bit PgmSz <- (#pc_v + $$ (* intwidth *) (natToWord PgmSz 1)) ;
         Retv ) (* rule decexecArith *)
-    with Rule instancePrefix--"decexecLd" :=
-    (
-        Read e2wFifo_valid_v : Bool <- e2wFifo_valid ;
-        Read pc_v : Bit PgmSz <- pc ;
-        Read sbFlags_v : Array NumRegs Bool <- sbFlags ;
-       Read instrs : Array NumInstrs (Bit InstrSz) <- pgm ;
-       LET call23 : Bit InstrSz <- #instrs @[ #pc_v ] ;
-       LET call22 : Bool <-  (getOp dec _ call23) == $$opLd ;
-       LET call25 : Bit InstrSz <-  #instrs @[ #pc_v ] ;
-       LET call24 : Bit RegFileSz <-  getDst dec _ call25 ;
-
-        Assert(((#call22 && (!(#sbFlags_v @[ #call24 ]))) && (!#e2wFifo_valid_v))) ;
-       LET inst : Bit InstrSz (* varbinding *) <- #instrs @[ #pc_v ] ;
-       LET src1 : Bit RegFileSz (* varbinding *) <-  getSrc1 dec _ inst ;
-       LET dst : Bit RegFileSz (* varbinding *) <-  getDst dec _ inst ;
-       LET addr : Bit AddrSz (* varbinding *) <- getAddr dec _ inst ;
-       Read regsval : Array NumRegs (Bit DataSz) <- rf ;
-       LET val1 : Bit DataSz (* varbinding *) <-  #regsval @[ #src1 ] ;
-
-               LET memrq : MemRq (* non-call varbinding *) <- STRUCT { "addr" ::= (#addr) ; "data" ::= (#val1) ; "isLoad" ::= ($$ (* intwidth *) (natToWord 1 1))  }%kami_expr ;
-               BKCall ldVal : Bit DataSz (* actionBinding *) <- mem'doMem ((#memrq) : MemRq) ;
-               LET flags : Array NumRegs Bool (* non-call varbinding *) <- #sbFlags_v ;
-               LET flags : Array NumRegs Bool <- #flags @[#dst <- $$true ] ;
-               Write sbFlags : Array NumRegs Bool <- #flags ;
-               LET e2w : E2W (* non-call varbinding *) <- STRUCT { "idx" ::= (#dst) ; "val" ::= (#ldVal)  }%kami_expr ;
-               Write e2wFifo_reg : E2W <- #e2w ;
-               Write e2wFifo_valid : Bool <- ($$true)%kami_expr ;
-               Write pc : Bit PgmSz <- (#pc_v + $$ (* intwidth *) (natToWord PgmSz 1)) ;
-        Retv ) (* rule decexecLd *)
-    with Rule instancePrefix--"decexecSt" :=
-    (
-        Read pc_v : Bit PgmSz <- pc ;
-       Read instrs : Array NumInstrs (Bit InstrSz) <- pgm ;
-       LET call27 : Bit InstrSz <-  #instrs @[ #pc_v ] ;
-       LET call26 : Bool <-  (getOp dec _ call27)  == $$opSt ;
-
-        Assert(#call26) ;
-       LET inst : Bit InstrSz (* varbinding *) <- #instrs @[ #pc_v ] ;
-       LET src1 : Bit RegFileSz (* varbinding *) <- getSrc1 dec _ inst ;
-       LET addr : Bit AddrSz (* varbinding *) <-  getAddr dec _ inst ;
-       Read regsval : Array NumRegs (Bit DataSz) <- rf ;
-       LET val1 : Bit DataSz (* varbinding *) <-  #regsval @[ #src1 ] ;
-               LET memrq : MemRq (* non-call varbinding *) <- STRUCT { "addr" ::= (#addr) ; "data" ::= (#val1) ; "isLoad" ::= ($$ (* intwidth *) (natToWord 1 0))  }%kami_expr ;
-               BKCall unused : Bit DataSz (* actionBinding *) <- mem'doMem ((#memrq) : MemRq) ;
-               Write pc : Bit PgmSz <- (#pc_v + $$ (* intwidth *) (natToWord PgmSz 1)) ;
-        Retv ) (* rule decexecSt *)
-    with Rule instancePrefix--"decexecToHost" :=
-    (
-        Read pc_v : Bit PgmSz <- pc ;
-        Read sbFlags_v : Array NumRegs Bool <- sbFlags ;
-       Read instrs : Array NumInstrs (Bit InstrSz) <- pgm ;
-       LET call29 : Bit InstrSz <-  #instrs @[  #pc_v ] ;
-       LET call28 : Bool <-  (getOp dec _ call29) == $$opTh ;
-       LET call31 : Bit InstrSz <-  #instrs @[ #pc_v ] ;
-       LET call30 : Bit RegFileSz <-  getSrc1 dec _ call31 ;
-
-        Assert((#call28 && (!(#sbFlags_v @[ #call30 ])))) ;
-       LET inst : Bit InstrSz (* varbinding *) <-  #instrs @[ #pc_v ] ;
-       LET src1 : Bit RegFileSz (* varbinding *) <- getSrc1 dec _ inst ;
-       Read regsval : Array NumRegs (Bit DataSz) <- rf ;
-       LET val1 : Bit DataSz (* varbinding *) <-  #regsval @[ #src1 ] ;
-
-               BKCall unused : Void (* actionBinding *) <- toHost'toHost ((#val1) : Bit DataSz) ;
-               Write pc : Bit PgmSz <- (#pc_v + $$ (* intwidth *) (natToWord PgmSz 1)) ;
-        Retv ) (* rule decexecToHost *)
     }). (* mkDecExec *)
 
     Hint Unfold mkDecExecModule : ModuleDefs.
@@ -164,7 +101,7 @@ Module module'mkDecExecSep.
     Let e2wFifo_reg : string := instancePrefix--"e2wFifo_reg".
     Let e2wFifo_valid : string := instancePrefix--"e2wFifo_valid".
     Let decoder_pc : string := instancePrefix--"pc".
-    Let sbFlags : string := instancePrefix--"sbFlags".
+    (* Let sbFlags : string := instancePrefix--"sbFlags". *)
     (* instance methods *)
     Let mem'doMem : string := mem--"doMem".
     Let toHost'toHost : string := toHost--"toHost".
@@ -179,7 +116,7 @@ Module module'mkDecExecSep.
     with Register e2wFifo_valid : Bool <- (false)%kami_expr
     with Register pgm : Array NumInstrs (Bit InstrSz) <- Default
     with Register rf : Array NumRegs (Bit DataSz) <- Default
-    with Register sbFlags : Array NumRegs Bool <- Default
+    (* with Register sbFlags : Array NumRegs Bool <- Default *)
     with Rule instancePrefix--"decode" :=
     (
         Read d2eFifo_valid_v : Bool <- d2eFifo_valid ;
@@ -205,11 +142,14 @@ Module module'mkDecExecSep.
     (
         Read d2eFifo_valid_v : Bool <- d2eFifo_valid ;
         Read e2wFifo_valid_v : Bool <- e2wFifo_valid ;
-        Read sbFlags_v : Array NumRegs Bool <- sbFlags ;
+        (* Read sbFlags_v : Array NumRegs Bool <- sbFlags ; *)
         Read d2eFifo_reg_v : D2E <- d2eFifo_reg ;
                LET d2e : D2E (* non-call varbinding *) <- #d2eFifo_reg_v ;
 
-        Assert(((((((#d2e @% "op") == $$ (* isConstT *)opArith) && (!(#sbFlags_v @[ (#d2e @% "src1") ]))) && (!(#sbFlags_v @[ (#d2e @% "src2") ]))) && #d2eFifo_valid_v) && (!#e2wFifo_valid_v))) ;
+        Assert( ((#d2e @% "op") == $$ (* isConstT *)opArith)
+	      (* && (!(#sbFlags_v @[ (#d2e @% "src1") ])) *)
+	      (*  && (!(#sbFlags_v @[ (#d2e @% "src2") ])) *)
+	       && #d2eFifo_valid_v && (!#e2wFifo_valid_v)) ;
                Write d2eFifo_valid : Bool <- ($$false)%kami_expr ;
                LET src1 : Bit RegFileSz (* non-call varbinding *) <- (#d2e @% "src1") ;
                LET src2 : Bit RegFileSz (* non-call varbinding *) <- (#d2e @% "src2") ;
@@ -220,71 +160,13 @@ Module module'mkDecExecSep.
        LET val2 : Bit DataSz (* varbinding *) <-  #regsval @[ #src2 ] ;
 
        LET execVal : Bit DataSz <- (execArith exec _ arithOp val1 val2) ;
-               LET flags : Array NumRegs Bool (* non-call varbinding *) <- #sbFlags_v ;
+               (* LET flags : Array NumRegs Bool (* non-call varbinding *) <- #sbFlags_v ;
                LET flags : Array NumRegs Bool <- #flags @[#dst <- $$true ] ;
-               Write sbFlags : Array NumRegs Bool <- #flags ;
+               Write sbFlags : Array NumRegs Bool <- #flags ; *)
                LET e2w : E2W (* non-call varbinding *) <- STRUCT { "idx" ::= (#dst) ; "val" ::= (#execVal)  }%kami_expr ;
                Write e2wFifo_reg : E2W <- #e2w ;
                Write e2wFifo_valid : Bool <- ($$true)%kami_expr ;
         Retv ) (* rule executeArith *)
-    with Rule instancePrefix--"executeLoad" :=
-    (
-        Read d2eFifo_valid_v : Bool <- d2eFifo_valid ;
-        Read e2wFifo_valid_v : Bool <- e2wFifo_valid ;
-        Read sbFlags_v : Array NumRegs Bool <- sbFlags ;
-        Read d2eFifo_reg_v : D2E <- d2eFifo_reg ;
-               LET d2e : D2E (* non-call varbinding *) <- #d2eFifo_reg_v ;
-
-        Assert(((((((#d2e @% "op") == $$ (* isConstT *)opLd) && (!(#sbFlags_v @[ (#d2e @% "src1") ]))) && (!(#sbFlags_v @[ (#d2e @% "dst") ]))) && #d2eFifo_valid_v) && (!#e2wFifo_valid_v))) ;
-               Write d2eFifo_valid : Bool <- ($$false)%kami_expr ;
-               LET src1 : Bit RegFileSz (* non-call varbinding *) <- (#d2e @% "src1") ;
-               LET dst : Bit RegFileSz (* non-call varbinding *) <- (#d2e @% "dst") ;
-               LET addr : Bit AddrSz (* non-call varbinding *) <- (#d2e @% "addr") ;
-       Read regsval : Array NumRegs (Bit DataSz) <- rf ;
-       LET val1 : Bit DataSz (* varbinding *) <-  #regsval @[ #src1 ] ;
-
-               LET memrq : MemRq (* non-call varbinding *) <- STRUCT { "addr" ::= (#addr) ; "data" ::= ($$ (* intwidth *) (natToWord 32 0)) ; "isLoad" ::= ($$ (* intwidth *) (natToWord 1 1))  }%kami_expr ;
-               BKCall ldVal : Bit DataSz (* actionBinding *) <- mem'doMem ((#memrq) : MemRq) ;
-               LET flags : Array NumRegs Bool (* non-call varbinding *) <- #sbFlags_v ;
-               LET flags : Array NumRegs Bool <- #flags @[ #dst <- $$true ] ;
-               Write sbFlags : Array NumRegs Bool <- #flags ;
-               LET e2w : E2W (* non-call varbinding *) <- STRUCT { "idx" ::= (#dst) ; "val" ::= (#ldVal)  }%kami_expr ;
-               Write e2wFifo_reg : E2W <- #e2w ;
-               Write e2wFifo_valid : Bool <- ($$true)%kami_expr ;
-        Retv ) (* rule executeLoad *)
-    with Rule instancePrefix--"executeStore" :=
-    (
-        Read d2eFifo_valid_v : Bool <- d2eFifo_valid ;
-        Read sbFlags_v : Array NumRegs Bool <- sbFlags ;
-        Read d2eFifo_reg_v : D2E <- d2eFifo_reg ;
-               LET d2e : D2E (* non-call varbinding *) <- #d2eFifo_reg_v ;
-
-        Assert(((((#d2e @% "op") == $$ (* isConstT *)opSt) && (!(#sbFlags_v @[ (#d2e @% "src1") ]))) && #d2eFifo_valid_v)) ;
-               Write d2eFifo_valid : Bool <- ($$false)%kami_expr ;
-               LET src1 : Bit RegFileSz (* non-call varbinding *) <- (#d2e @% "src1") ;
-               LET addr : Bit AddrSz (* non-call varbinding *) <- (#d2e @% "addr") ;
-       Read regsval : Array NumRegs (Bit DataSz) <- rf ;
-       LET val1 : Bit DataSz (* varbinding *) <-  #regsval @[ #src1 ] ;
-
-               LET memrq : MemRq (* non-call varbinding *) <- STRUCT { "addr" ::= (#addr) ; "data" ::= (#val1) ; "isLoad" ::= ($$ (* intwidth *) (natToWord 1 0))  }%kami_expr ;
-               BKCall unused : Bit DataSz (* actionBinding *) <- mem'doMem ((#memrq) : MemRq) ;
-        Retv ) (* rule executeStore *)
-    with Rule instancePrefix--"executeToHost" :=
-    (
-        Read d2eFifo_valid_v : Bool <- d2eFifo_valid ;
-        Read sbFlags_v : Array NumRegs Bool <- sbFlags ;
-        Read d2eFifo_reg_v : D2E <- d2eFifo_reg ;
-               LET d2e : D2E (* non-call varbinding *) <- #d2eFifo_reg_v ;
-
-        Assert(((((#d2e @% "op") == $$ (* isConstT *)opTh) && (!(#sbFlags_v @[ (#d2e @% "src1") ]))) && #d2eFifo_valid_v)) ;
-               Write d2eFifo_valid : Bool <- ($$false)%kami_expr ;
-               LET src1 : Bit RegFileSz (* non-call varbinding *) <- (#d2e @% "src1") ;
-               LET addr : Bit AddrSz (* non-call varbinding *) <- (#d2e @% "addr") ;
-       Read regsval : Array NumRegs (Bit DataSz) <- rf ;
-       LET val1 : Bit DataSz (* varbinding *) <-  #regsval @[ #src1 ] ;
-
-               BKCall unused : Void (* actionBinding *) <- toHost'toHost ((#val1) : Bit DataSz) ;
-        Retv ) (* rule executeToHost *)
     }). (* mkDecExecSep *)
 
     Hint Unfold mkDecExecSepModule : ModuleDefs.
